Calculus/MultiStaged/Translation.v
@@ -2,9 +2,11 @@ Require Import Coq.Lists.List.
 Require Import Coq.Arith.Arith.
 Require Import Coq.Relations.Relation_Definitions.
 Require Import "Misc/Library".
+Require Import "Misc/Tactics".
 Require Import "Calculus/Sets".
 Require Import "Calculus/Definitions".
 Require Import "Calculus/MultiStaged/Definitions".
+Require Import "Calculus/MultiStaged/DataGathering".
 Require Import "Calculus/MultiStaged/Monad".
 
 (**
@@ -20,10 +22,11 @@ Definition hole_var (x:nat) : nat := (2*x+1)%nat.
 Definition source_var (x:nat) : nat := (2*x)%nat.
 
 Module Type Context (R:Replacement) (S:ReplacementCalculus R) 
-  (T:StagedCalculus) (M:Monad R S T).
+  (T:StagedCalculus) (DG:DataGathering R S) (M:Monad R S T DG).
 
   Import T.
   Import M.
+  Import DG.
 
   Definition t : Type := list (expr * S.var).
   Definition t_stack : Type := list t.
@@ -104,16 +107,21 @@ Module Type Context (R:Replacement) (S:ReplacementCalculus R)
 End Context.
 
 Module ContextImpl (R:Replacement) (S:ReplacementCalculus R) 
-    (T:StagedCalculus) (M:Monad R S T) : Context R S T M.
-  Include Context R S T M.
+    (T:StagedCalculus) (DG:DataGathering R S) (M:Monad R S T DG) : 
+    Context R S T DG M.
+  Include Context R S T DG M.
 End ContextImpl.
 
 (* Translation R S T <: StagedTranslation S T. *)
 Module Type Translation (R:Replacement) (S:ReplacementCalculus R)
-    (T:StagedCalculus) (M:Monad R S T). 
+    (T:StagedCalculus) (DG:DataGathering R S) 
+    (DGP:DataGatheringPredicates R S DG)
+    (DGR:DataGatheringRequirements R S DG DGP) (M:Monad R S T DG). 
 
-  Module Context := ContextImpl R S T M.
+  Module Context := ContextImpl R S T DG M.
+  Module DGValid := DataGatheringProperties R S DG DGP DGR.
   Import S.CRaw.
+  Import DG.
 
   Fixpoint booker (e:S.expr) (n:nat) : nat :=
     match e with 
@@ -138,88 +146,88 @@ Module Type Translation (R:Replacement) (S:ReplacementCalculus R)
   Definition map_iter_booker (e:S.expr) (bs:list nat) (n:nat) :=
     List2.map_iter (fun b n => (b+booker e n)%nat) bs n.
 
-  Fixpoint trans (e:S.expr) (bs:list nat) (dg:M.dg_t) (dgs:list M.dg_t) : T.expr * Context.t_stack :=
+  Fixpoint trans (e:S.expr) (bs:list nat) (dg:dg_t) (dgs:list dg_t) : T.expr * Context.t_stack :=
     match e with
     | EConst i => (M.ret dg (M.cast_econst dg i), Context.empty)
     | EVar y => (M.ret dg (M.cast_evar dg (M.cast_var (source_var y))), Context.empty)
     | EAbs y e => 
-        let (e,cs) := trans e bs (M.dg_eabs dg y) dgs in
+        let (e,cs) := trans e bs (dg_eabs dg y) dgs in
         (M.ret dg (M.cast_eabs dg (M.cast_var (source_var y)) e), cs)
     | EFix f y e => 
-        let (e,cs) := trans e bs (M.dg_efix dg f y) dgs in
+        let (e,cs) := trans e bs (dg_efix dg f y) dgs in
         (M.ret dg (M.cast_efix dg
             (M.cast_var (source_var f)) 
             (M.cast_var (source_var y)) e), cs)
     | EApp e1 e2 => 
         let bs2 := map_iter_booker e2 bs 0 in
-        let (e1', cs1) := trans e1 bs2 (M.dg_eapp_l dg) dgs in
-        let (e2', cs2) := trans e2 bs (M.dg_eapp_r dg) dgs in
+        let (e1', cs1) := trans e1 bs2 (dg_eapp_l dg) dgs in
+        let (e2', cs2) := trans e2 bs (dg_eapp_r dg) dgs in
           (if svalueb 0 e1 then
 	   M.bind dg e2' (fun v2 => M.cast_eapp dg 
-             (phi e1 bs2 (M.dg_eapp_l dg) dgs) v2)
+             (phi e1 bs2 (dg_eapp_l dg) dgs) v2)
 	   else M.bind dg e1' (fun v1 => M.bind dg e2'
           (fun v2 => M.cast_eapp dg v1 v2)), 
           Context.merge cs1 cs2)
     | ELoc l => (M.ret dg (M.cast_eloc dg l), Context.empty)
     | ERef e => 
-        let (e,cs) := trans e bs (M.dg_eref dg) dgs in
+        let (e,cs) := trans e bs (dg_eref dg) dgs in
         (M.bind dg e (fun v => M.cast_eref dg v), cs)
     | EDeref e => 
-        let (e,cs) := trans e bs (M.dg_ederef dg) dgs in
+        let (e,cs) := trans e bs (dg_ederef dg) dgs in
         (M.bind dg e (fun v => M.cast_ederef dg v), cs)
     | EAssign e1 e2 => 
 	let bs2 := map_iter_booker e2 bs 0 in
-        let (e1', cs1) := trans e1 bs2 (M.dg_eassign_l dg) dgs in
-        let (e2', cs2) := trans e2 bs (M.dg_eassign_r dg) dgs in
+        let (e1', cs1) := trans e1 bs2 (dg_eassign_l dg) dgs in
+        let (e2', cs2) := trans e2 bs (dg_eassign_r dg) dgs in
           (if svalueb 0 e1 then
 	   M.bind dg e2' (fun v2 => M.cast_eassign dg 
-             (phi e1 bs2 (M.dg_eassign_l dg) dgs) v2)
+             (phi e1 bs2 (dg_eassign_l dg) dgs) v2)
 	   else M.bind dg e1' (fun v1 => M.bind dg e2'
           (fun v2 => M.cast_eassign dg v1 v2)), 
           Context.merge cs1 cs2)
     | EBox e => 
-        let (e, cs) := trans e (0 :: bs) (M.dg_ebox dg) (dg::dgs) in
+        let (e, cs) := trans e (0 :: bs) (dg_ebox dg) (dg::dgs) in
         match cs with
         | nil => (M.ret dg (M.cast_ebox dg e), Context.empty)
         | c :: cs => (Context.fill dg c (M.ret dg (M.cast_ebox dg e)), cs)
         end
     | EUnbox e =>
         let (b, bs) := List2.hd_cons bs 0 in
-        let (dg', dgs') := List2.hd_cons dgs M.dg_empty in
+        let (dg', dgs') := List2.hd_cons dgs dg_empty in
         let (e', cs) := trans e bs dg' dgs' in
            (M.cast_eunbox dg (M.cast_evar dg 
 	   (M.cast_var (hole_var b))), ((e', b) :: nil) :: cs)
     | ERun e =>
-        let (e,cs) := trans e bs (M.dg_erun dg) dgs in
+        let (e,cs) := trans e bs (dg_erun dg) dgs in
         (M.bind dg e (fun v => M.cast_erun dg v), cs)
     | ELift e =>
-        let (e,cs) := trans e bs (M.dg_elift dg) dgs in
+        let (e,cs) := trans e bs (dg_elift dg) dgs in
         (M.bind dg e (fun v => M.cast_elift dg v), cs)
     end
 
-  with phi (e:S.expr) (bs:list nat) (dg:M.dg_t) (dgs:list M.dg_t) : T.expr :=
+  with phi (e:S.expr) (bs:list nat) (dg:dg_t) (dgs:list dg_t) : T.expr :=
     match e with
     | EConst i => M.cast_econst dg i
     | EVar y => M.cast_evar dg (M.cast_var (source_var y))
     | EAbs y e => 
-        let (e, _) := trans e bs (M.dg_eabs dg y) dgs in
+        let (e, _) := trans e bs (dg_eabs dg y) dgs in
         M.cast_eabs dg (M.cast_var (source_var y)) e
     | EFix f y e => 
-        let (e, _) := trans e bs (M.dg_efix dg f y) dgs in
+        let (e, _) := trans e bs (dg_efix dg f y) dgs in
         M.cast_efix dg
             (M.cast_var (source_var f)) 
             (M.cast_var (source_var y)) e
     | ELoc l => M.cast_eloc dg l
     | EBox e => 
-        let (e, _) := trans e (0 :: bs) (M.dg_ebox dg) (dg::dgs) in
+        let (e, _) := trans e (0 :: bs) (dg_ebox dg) (dg::dgs) in
         M.cast_ebox dg e
     | _ => M.cast_econst dg 0
     end.
 
-  Definition trans_expr (e:S.expr) (bs:list nat) (dg:M.dg_t) (dgs:list M.dg_t) : T.expr :=
+  Definition trans_expr (e:S.expr) (bs:list nat) (dg:dg_t) (dgs:list dg_t) : T.expr :=
     let (e, _) := trans e bs dg dgs in e.
 
-  Fixpoint trans_mem (m:S.Memory.t) (bs:list nat) (dg:M.dg_t) (dgs:list M.dg_t) : T.Memory.t :=
+  Fixpoint trans_mem (m:S.Memory.t) (bs:list nat) (dg:dg_t) (dgs:list dg_t) : T.Memory.t :=
     match m with
     | nil => nil
     | e :: m => (phi e bs dg dgs) :: (trans_mem m bs dg dgs)
@@ -230,46 +238,47 @@ Module Type Translation (R:Replacement) (S:ReplacementCalculus R)
     | Admin_refl : forall (e:T.expr), admin e e
     | Admin_trans : forall (e1 e2 e3:T.expr), 
         admin e1 e2 -> admin e2 e3 -> admin e1 e3
-    | Admin_abs : forall (x:T.var) (e1 e2:T.expr) (dg:M.dg_t),
+    | Admin_abs : forall (x:T.var) (e1 e2:T.expr) (dg:dg_t),
         admin e1 e2 -> admin (M.cast_eabs dg x e1) (M.cast_eabs dg x e2)
-    | Admin_fix : forall (f x:T.var) (e1 e2:T.expr) (dg:M.dg_t),
+    | Admin_fix : forall (f x:T.var) (e1 e2:T.expr) (dg:dg_t),
         admin e1 e2 -> admin (M.cast_efix dg f x e1) (M.cast_efix dg f x e2)
-    | Admin_app : forall (e1 e2 e3 e4:T.expr) (dg:M.dg_t),
+    | Admin_app : forall (e1 e2 e3 e4:T.expr) (dg:dg_t),
         admin e1 e3 -> admin e2 e4 -> 
         admin (M.cast_eapp dg e1 e2) (M.cast_eapp dg e3 e4)
-    | Admin_ref : forall (e1 e2:T.expr) (dg:M.dg_t),
+    | Admin_ref : forall (e1 e2:T.expr) (dg:dg_t),
         admin e1 e2 -> admin (M.cast_eref dg e1) (M.cast_eref dg e2)
-    | Admin_deref : forall (e1 e2:T.expr) (dg:M.dg_t),
+    | Admin_deref : forall (e1 e2:T.expr) (dg:dg_t),
         admin e1 e2 -> admin (M.cast_ederef dg e1) (M.cast_ederef dg e2)
-    | Admin_assign : forall (e1 e2 e3 e4:T.expr) (dg:M.dg_t),
+    | Admin_assign : forall (e1 e2 e3 e4:T.expr) (dg:dg_t),
         admin e1 e3 -> admin e2 e4 -> 
         admin (M.cast_eassign dg e1 e2) (M.cast_eassign dg e3 e4)
-    | Admin_box : forall (e1 e2:T.expr) (dg:M.dg_t),
+    | Admin_box : forall (e1 e2:T.expr) (dg:dg_t),
         admin e1 e2 -> admin (M.cast_ebox dg e1) (M.cast_ebox dg e2)
-    | Admin_unbox : forall (e1 e2:T.expr) (dg:M.dg_t),
+    | Admin_unbox : forall (e1 e2:T.expr) (dg:dg_t),
         admin e1 e2 -> admin (M.cast_eunbox dg e1) (M.cast_eunbox dg e2)
-    | Admin_run : forall (e1 e2:T.expr) (dg:M.dg_t),
+    | Admin_run : forall (e1 e2:T.expr) (dg:dg_t),
         admin e1 e2 -> admin (M.cast_erun dg e1) (M.cast_erun dg e2)
-    | Admin_lift : forall (e1 e2:T.expr) (dg:M.dg_t),
+    | Admin_lift : forall (e1 e2:T.expr) (dg:dg_t),
         admin e1 e2 -> admin (M.cast_elift dg e1) (M.cast_elift dg e2)
-    | Admin_ret : forall (e1 e2:T.expr) (dg:M.dg_t),
+    | Admin_ret : forall (e1 e2:T.expr) (dg:dg_t),
         admin e1 e2 -> admin (M.ret dg e1) (M.ret dg e2)
-    | Admin_bind : forall (e1 e2:T.expr) (f1 f2:T.expr -> T.expr) (dg:M.dg_t),
+    | Admin_bind : forall (e1 e2:T.expr) (f1 f2:T.expr -> T.expr) (dg:dg_t),
         admin e1 e2 -> (forall e3:T.expr, admin (f1 e3) (f2 e3)) ->
         admin (M.bind dg e1 f1) (M.bind dg e2 f2)
-   | Admin_unbox_box : forall (e:expr) (bs:list nat) (dg:M.dg_t) (dgs:list M.dg_t),
+   | Admin_unbox_box : forall (e:expr) (*(bs:list nat)*) (dg:dg_t) (dgs:list dg_t),
         svalue 1 e ->
-        admin (M.cast_eunbox dg (M.cast_ebox dg 
-          (trans_expr e bs dg dgs))) 
-          (trans_expr e bs dg dgs)
-   | Admin_bind_app_phi : forall (v:expr) (e:T.expr) (bs:list nat) (dg:M.dg_t) (dgs:list M.dg_t), 
-       svalue 0 v ->
+        DGValid.valid_dgs 1 dg (dg_empty :: dgs) ->
+        admin (M.cast_eunbox dg (M.cast_ebox dg_empty
+          (trans_expr e (0::nil) dg (dg_empty :: dgs)))) 
+          (trans_expr e (0::nil) dg (dg_empty :: dgs))
+   | Admin_bind_app_phi : forall (v:expr) (e:T.expr) (bs:list nat) (dg:dg_t) (dgs:list dg_t), 
+       svalue 0 v -> 
        let f := fun v0 => M.bind dg e (fun v1 => M.cast_eapp dg v0 v1) in
-       admin (M.bind dg (M.ret (M.dg_eapp_l dg) (phi v bs (M.dg_eapp_l dg) dgs)) f) (f (phi v bs (M.dg_eapp_l dg) dgs))
-  | Admin_bind_assign_phi : forall (v:expr) (e:T.expr) (bs:list nat) (dg:M.dg_t) (dgs:list M.dg_t), 
+       admin (M.bind dg (M.ret (dg_eapp_l dg) (phi v bs (dg_eapp_l dg) dgs)) f) (f (phi v bs (dg_eapp_l dg) dgs))
+  | Admin_bind_assign_phi : forall (v:expr) (e:T.expr) (bs:list nat) (dg:dg_t) (dgs:list dg_t), 
        svalue 0 v ->
        let f := fun v0 => M.bind dg e (fun v1 => M.cast_eassign dg v0 v1) in
-       admin (M.bind dg (M.ret (M.dg_eassign_l dg) (phi v bs (M.dg_eassign_l dg) dgs)) f) (f (phi v bs (M.dg_eassign_l dg) dgs)).
+       admin (M.bind dg (M.ret (dg_eassign_l dg) (phi v bs (dg_eassign_l dg) dgs)) f) (f (phi v bs (dg_eassign_l dg) dgs)).
 
   Definition admin_context :  relation Context.t := 
     Context.congr_context admin.
@@ -284,6 +293,9 @@ Module Type Translation (R:Replacement) (S:ReplacementCalculus R)
 End Translation.
 
 Module TranslationImpl (R:Replacement) 
-   (S:ReplacementCalculus R) (T:StagedCalculus) (M:Monad R S T). 
-  Include Translation R S T M.
+   (S:ReplacementCalculus R) (T:StagedCalculus) 
+   (DG:DataGathering R S) (DGP:DataGatheringPredicates R S DG)  
+   (DGR:DataGatheringRequirements R S DG DGP) 
+   (M:Monad R S T DG) <: Translation R S T DG DGP DGR M.
+  Include Translation R S T DG DGP DGR M.
 End TranslationImpl.
