Calculus/MultiStaged/DataGathering.v
@@ -1,0 +1,269 @@
+Require Import Coq.Lists.List.
+Require Import Coq.Arith.Arith.
+Require Import Coq.Relations.Relation_Definitions.
+Require Import "Misc/Tactics".
+Require Import "Calculus/Sets".
+Require Import "Calculus/Definitions".
+Require Import "Calculus/Monad".
+Require Import "Calculus/MultiStaged/Definitions".
+
+Module Type DataGathering (R:Replacement) 
+  (S:ReplacementCalculus R).
+
+  Parameter dg_t: Type.
+  Parameter dg_empty: dg_t.
+  Parameter dg_eabs: dg_t -> S.var -> dg_t.
+  Parameter dg_efix: dg_t -> S.var -> S.var -> dg_t.
+  Parameter dg_eapp_l: dg_t -> dg_t.
+  Parameter dg_eapp_r: dg_t -> dg_t.
+  Parameter dg_eref: dg_t -> dg_t.
+  Parameter dg_ederef: dg_t -> dg_t.
+  Parameter dg_eassign_l: dg_t -> dg_t.
+  Parameter dg_eassign_r: dg_t -> dg_t.
+  Parameter dg_erun: dg_t -> dg_t.
+  Parameter dg_elift: dg_t -> dg_t.
+  Parameter dg_ebox: dg_t -> dg_t.
+
+End DataGathering.
+
+Module Type DataGatheringPredicates (R:Replacement) 
+  (S:ReplacementCalculus R) (DG:DataGathering R S).
+
+  Import DG.
+
+  (**
+  All predicates aim to express well-formness properties
+  of data gathering values. As we have no information
+  about data gathering types, we need those properties
+  in a quite complicated way, controlling the tree
+  of applications of abstract operations over those types.
+  *)
+
+  (**
+  dg_comp dg1 dg2 is true iff dg2 is resulting from dg1
+  by composing it with arbitrary number of dg_.. operations.
+  *)
+  Inductive dg_comp : dg_t -> dg_t -> Prop :=
+  | DgCompId : forall (dg:dg_t), dg_comp dg dg
+  | DgCompEAbs : forall (dg1 dg2:dg_t) (x:S.var),
+    dg_comp dg1 dg2 -> dg_comp dg1 (dg_eabs dg2 x)
+  | DgCompEFix : forall (dg1 dg2:dg_t) (f x:S.var),
+    dg_comp dg1 dg2 -> dg_comp dg1 (dg_efix dg2 f x)
+  | DgCompEAppL : forall (dg1 dg2:dg_t),
+    dg_comp dg1 dg2 -> dg_comp dg1 (dg_eapp_l dg2)
+  | DgCompEAppR : forall (dg1 dg2:dg_t),
+    dg_comp dg1 dg2 -> dg_comp dg1 (dg_eapp_r dg2)
+  | DgCompERef : forall (dg1 dg2:dg_t),
+    dg_comp dg1 dg2 -> dg_comp dg1 (dg_eref dg2)
+  | DgCompEDeref : forall (dg1 dg2:dg_t),
+    dg_comp dg1 dg2 -> dg_comp dg1 (dg_ederef dg2)
+  | DgCompEAssignL : forall (dg1 dg2:dg_t),
+    dg_comp dg1 dg2 -> dg_comp dg1 (dg_eassign_l dg2)
+  | DgCompEAssignR : forall (dg1 dg2:dg_t),
+    dg_comp dg1 dg2 -> dg_comp dg1 (dg_eassign_r dg2)
+  | DgCompERun : forall (dg1 dg2:dg_t),
+    dg_comp dg1 dg2 -> dg_comp dg1 (dg_erun dg2)
+  | DgCompELift : forall (dg1 dg2:dg_t),
+    dg_comp dg1 dg2 -> dg_comp dg1 (dg_elift dg2).
+
+  (**
+  dg_comp_lst is the list closure of dg_comp. It checks pairwise
+  wether elements of lists are obtained from each other
+  by arbitrary composition of dg_... operations.
+  *)
+  Inductive dg_comp_lst (dg:dg_t) : (list dg_t) -> Prop :=
+  | DgCompLstNil : dg_comp_lst dg nil
+  | DgCompLstCons : forall (dg1:dg_t) (dgs:list dg_t),
+    dg_comp_lst dg1 dgs -> dg_comp (dg_ebox dg1) dg -> dg_comp_lst dg (dg1::dgs).
+
+  (**
+  dg_nth_empty dg n checks whether dg is obtained
+  by applying n occurrences of dg_ebox (modulo dg_comp).
+  *)
+  Inductive dg_nth_empty : dg_t -> nat -> Prop :=
+  | DgNthEmpty0 : dg_nth_empty dg_empty 0
+  | DgNthEmptyS : forall (dg1 dg2:dg_t) (n:nat),
+      dg_nth_empty dg1 n -> dg_comp (dg_ebox dg1) dg2 -> 
+      dg_nth_empty dg2 (S n).
+
+End DataGatheringPredicates.
+
+Module Type DataGatheringRequirements (R:Replacement) 
+  (S:ReplacementCalculus R) (DG:DataGathering R S)
+  (DGP:DataGatheringPredicates R S DG).
+
+  Import DG.
+  Import DGP.
+
+  Parameter dg_eabs_empty : 
+    forall (x:S.var), dg_eabs dg_empty x = dg_empty.
+
+  Parameter dg_efix_empty :
+    forall (f x:S.var), dg_efix dg_empty f x = dg_empty.
+
+  Parameter dg_eapp_l_empty : dg_eapp_l dg_empty = dg_empty.
+  Parameter dg_eapp_r_empty : dg_eapp_r dg_empty = dg_empty.
+  Parameter dg_eref_empty : dg_eref dg_empty = dg_empty.
+  Parameter dg_ederef_empty : dg_ederef dg_empty = dg_empty.
+  Parameter dg_eassign_l_empty : dg_eassign_l dg_empty = dg_empty.
+  Parameter dg_eassign_r_empty : dg_eassign_r dg_empty = dg_empty.
+  Parameter dg_erun_empty : dg_erun dg_empty = dg_empty.
+  Parameter dg_elift_empty : dg_elift dg_empty = dg_empty.
+
+  Parameter dg_ebox_empty :
+    forall (dg:dg_t) (n:nat), R.rho (S n) = true ->
+    dg_nth_empty dg n -> dg_ebox dg = dg_empty.
+
+End DataGatheringRequirements.
+
+Module DataGatheringProperties (R:Replacement)
+  (S:ReplacementCalculus R) (DG:DataGathering R S) 
+  (DGP:DataGatheringPredicates R S DG)
+  (DGR:DataGatheringRequirements R S DG DGP).
+
+  Import DG.
+  Import DGP.
+  Import DGR.
+
+  Definition valid_dgs (n:nat) (dg:dg_t) (dgs:list dg_t) :=
+    n <= length dgs /\
+    dg_comp_lst dg dgs /\
+    forall (m:nat), m <= n -> R.rho m = true -> 
+    match (n - m) with
+    | 0 => dg = dg_empty
+    | S n => nth n dgs dg_empty = dg_empty
+    end.
+
+  Lemma dg_comp_trans:
+    forall (dg1 dg2 dg3:dg_t),
+    dg_comp dg1 dg2 -> dg_comp dg2 dg3 -> dg_comp dg1 dg3.
+  Proof.
+    intros ; generalize dependent dg1.
+    induction H0 ; intros ; auto ;
+    try(constructor ; auto ; fail).
+  Qed.
+
+  Lemma dg_comp_lst_trans:
+    forall (dg1 dg2:dg_t) (dgs:list dg_t),
+    dg_comp dg1 dg2 -> dg_comp_lst dg1 dgs -> dg_comp_lst dg2 dgs.
+  Proof.
+    intros ; generalize dependent dgs.
+    inverts H ; intros ; auto ;
+    try(destruct dgs ; inverts H1 ; constructor ; auto ;
+    apply dg_comp_trans with (dg2:=dg1) ; auto ;
+    constructor ; auto).
+  Qed.
+
+  Lemma dg_comp_empty_ind:
+    forall (dg1 dg2:dg_t), dg_comp dg1 dg2 -> dg1 = dg_empty -> dg2 = dg_empty.
+  Proof.
+    assert(dg_empty = dg_empty) as Eq1.
+    reflexivity.
+
+    intros ; induction H ; subst ; auto ~ ;
+    specialize (IHdg_comp Eq1) ; subst.
+    apply dg_eabs_empty.
+    apply dg_efix_empty.
+    apply dg_eapp_l_empty.
+    apply dg_eapp_r_empty.
+    apply dg_eref_empty.
+    apply dg_ederef_empty.
+    apply dg_eassign_l_empty.
+    apply dg_eassign_r_empty.
+    apply dg_erun_empty.
+    apply dg_elift_empty.
+  Qed.
+
+  Lemma dg_comp_empty:
+    forall (dg:dg_t), dg_comp dg_empty dg -> dg = dg_empty.
+  Proof.
+     intros ; apply dg_comp_empty_ind with (dg1:=dg_empty) ; auto ~.
+  Qed.
+
+  Lemma valid_dgs_trans:
+    forall (n:nat) (dg1 dg2:dg_t) (dgs:list dg_t),
+    dg_comp dg1 dg2 -> valid_dgs n dg1 dgs -> valid_dgs n dg2 dgs.
+  Proof.
+    unfold valid_dgs ; intros ; repeat(split) ; auto ~ ; intros.
+    destruct H0 ; auto ~.
+    destruct H0 ; destruct H1.
+    apply dg_comp_lst_trans with (dg1:=dg1) ; auto ~.
+    destruct H0 ; destruct H3.
+    specialize (H4 m H1 H2).
+    destruct (n-m) ; subst ; auto ~.
+    apply dg_comp_empty ; auto ~.
+  Qed.
+
+  Lemma valid_dgs_eunbox:
+    forall (n:nat) (dg1 dg2:dg_t) (dgs:list dg_t),
+    valid_dgs (S n) dg1 (dg2::dgs) -> valid_dgs n dg2 dgs.
+  Proof.
+    unfold valid_dgs ; intros ; repeat(split) ; auto ~ ; intros.
+    destruct H ; simpl in *|-* ; omega.
+    destruct H ; destruct H0 ; inverts H0 ; auto ~.
+    destruct H ; destruct H2.
+    assert(m <= S n) as Eq1.
+    omega.
+    specialize (H3 m Eq1 H1).
+    rewrite <- minus_Sn_m in H3 ; auto ~.
+    destruct (n - m) ; auto ~.
+  Qed.
+
+  Lemma dg_nth_empty_lst:
+    forall (n:nat) (dg:dg_t) (dgs:list dg_t),
+    length dgs >= n ->
+    dg_comp_lst dg dgs ->
+    nth n (dg::dgs) dg_empty = dg_empty -> 
+    dg_nth_empty dg n.
+  Proof.
+    induction n ; simpl ; intros.
+    subst ; constructor.
+    destruct dgs.
+    exfalso ; simpl in *|-* ; omega.
+    simpl in H ; apply le_S_n in H.
+    inverts H0.
+    specialize (IHn d dgs H H4).
+    apply DgNthEmptyS with (dg1:=d) ; auto ~.
+  Qed.
+
+  Lemma valid_dgs_ebox:
+    forall (n:nat) (dg:dg_t) (dgs:list dg_t),
+    valid_dgs n dg dgs -> valid_dgs (S n) (dg_ebox dg) (dg :: dgs).
+  Proof.
+    unfold valid_dgs ; intros ; repeat(split) ; auto ~ ; intros.
+    simpl ; omega.
+    destruct H ; destruct H0 ; constructor ; auto ~ ; repeat(constructor).
+    case_beq_nat m (S n).
+    rewrite minus_diag.
+    apply dg_ebox_empty with (n:=n) ; auto ~.
+    destruct H ; destruct H2.
+    assert(0 <= n) as Eq1.
+    omega.
+    specialize (H3 0 Eq1 R.rho_O).
+    apply dg_nth_empty_lst with (dgs:=dgs) ; auto ~.
+    rewrite <- minus_n_O in H3 ; destruct n ; auto ~.
+    assert(m <= n) as Eq1.
+    omega.
+    rewrite <- minus_Sn_m ; auto ~.
+    destruct H ; destruct H2 ; specialize (H3 m Eq1 H1).
+    destruct (n-m) ; auto ~.
+  Qed.
+
+  Lemma dg_valid_dgs_nil: valid_dgs 0 dg_empty nil.
+  Proof.
+    repeat(split) ; intros ; auto ~.
+    constructor.
+  Qed.
+
+  Lemma dg_valid_dgs_empty: 
+    forall (dg:dg_t) (dgs:list dg_t),
+    valid_dgs 0 dg dgs -> dg = dg_empty.
+  Proof.
+    intros ; destruct H.
+    destruct H0.
+    specialize (H1 0) ; simpl in *|-*.
+    apply H1 ; auto.
+    apply R.rho_O.
+  Qed.
+  
+End DataGatheringProperties.
